x86/Asmlabelgenproof.v
@@ -9,7 +9,7 @@
 Require Import Coqlib Errors.
 Require Import Integers Floats AST Linking.
 Require Import Values Memory Events Globalenvs Smallstep.
-Require Import Op Locations Mach Conventions Asm.
+Require Import Op Locations Mach Conventions Asm RealAsm.
 Require Import Asmlabelgen.
 Import ListNotations.
 Require AsmFacts.
@@ -40,13 +40,12 @@ Let ge := Genv.globalenv prog.
 Let tge := Genv.globalenv tprog.
 
 Hypothesis TRANSF: match_prog prog tprog.
-Hypothesis TRANSF_PROG: transf_program prog = OK tprog.
 
 Inductive match_states : Asm.state -> Asm.state -> Prop :=
 |match_states_intro m rs:
    match_states (Asm.State rs m) (Asm.State rs m).
 
-Variable init_stk: stack.
+(* Variable init_stk: stack. *)
 
 
 
@@ -328,18 +327,17 @@ Proof.
     simpl. auto.
   + unfold offsets_after_call.
     unfold transl_code in HTrans.
-    setoid_rewrite (fold_left_app _ [a] c) in HTrans.
-    
-  unfold offsets_after_call.
+    setoid_rewrite (fold_left_app _ [a] c) in HTrans.    
+    unfold offsets_after_call.
 
 Admitted.
 
 
 
 Theorem step_simulation:
-  forall S1 t S2, step init_stk ge S1 t S2 ->
+  forall S1 t S2, step ge S1 t S2 ->
                   forall S1' (MS: match_states S1 S1'),
-                    (exists S2', step init_stk tge S1' t S2' /\ match_states S2 S2').
+                    (exists S2', step tge S1' t S2' /\ match_states S2 S2').
 Proof.
   intros S1 t S2 HStep S1' MS.
   inversion MS.
@@ -633,29 +631,30 @@ Proof.
       repeat rewrite Z.add_assoc.
       omega.
       admit. admit. admit. admit. admit.
-      
-    +++ subst. rewrite H4.
 
-      Lemma check_ra_after_call_eq : forall v a b,
-        check_ra_after_call ge v = left a <-> check_ra_after_call tge v = left b.
-      Admitted.
+    +++ admit.
+    (* +++ subst. rewrite H4. *)
 
-      destruct check_ra_after_call eqn:N; try congruence.
-      rewrite check_ra_after_call_eq in N. unfold tge in N.
-      rewrite N.
-      destruct (Mem.check_top_tc m); inversion H4.
-      auto.
+    (*   Lemma check_ra_after_call_eq : forall v a b, *)
+    (*     check_ra_after_call ge v = left a <-> check_ra_after_call tge v = left b. *)
+    (*   Admitted. *)
+
+    (*   destruct check_ra_after_call eqn:N; try congruence. *)
+    (*   rewrite check_ra_after_call_eq in N. unfold tge in N. *)
+    (*   rewrite N. *)
+    (*   destruct (Mem.check_top_tc m); inversion H4. *)
+    (*   auto. *)
                                                     
-      (* Lemma transf_ra_refl: forall v, *)
-      (*   ra_after_call ge v = ra_after_call tge v. *)
-      (* Admitted. *)
+    (*   (* Lemma transf_ra_refl: forall v, *) *)
+    (*   (*   ra_after_call ge v = ra_after_call tge v. *) *)
+    (*   (* Admitted. *) *)
       
-      (* destruct (check_ra_after_call (Genv.globalenv tprog) (rs RA)) eqn:EQRA. *)
-      (* destruct (check_ra_after_call ge (rs RA)) eqn:EQRA'. *)
-      (* auto. *)
-      (* generalize (transf_ra_refl (rs RA)). *)
-      (* intros HRA. *)
-      (* destruct (Mem.check_top_tc m); inversion H4. *)
+    (*   (* destruct (check_ra_after_call (Genv.globalenv tprog) (rs RA)) eqn:EQRA. *) *)
+    (*   (* destruct (check_ra_after_call ge (rs RA)) eqn:EQRA'. *) *)
+    (*   (* auto. *) *)
+    (*   (* generalize (transf_ra_refl (rs RA)). *) *)
+    (*   (* intros HRA. *) *)
+    (*   (* destruct (Mem.check_top_tc m); inversion H4. *) *)
           
   ++
     generalize(Genv.find_funct_ptr_transf_partial TRANSF _  H2).
@@ -685,44 +684,84 @@ Proof.
     eapply exec_step_external; eauto.
     apply external_call_symbols_preserved with (ge1:=ge); eauto.
     eapply Genv.senv_transf_partial; eauto.
-    unfold ra_after_call.
-    unfold ra_after_call in H7.
-    destruct H7 as (HRA & HRAP).
-    split.
-    +++ inversion H. auto.
-    +++ intros b0 o HRAPointer f HFindF.
-        generalize (HRAP _ _ HRAPointer). intro FACALL.
-
-        destruct (Genv.find_funct_ptr ge b0) eqn:FPTR1.
-        generalize (FACALL _ eq_refl). intros FACALL1.
-        generalize (Genv.find_funct_ptr_transf_partial TRANSF _ FPTR1).
-        destruct 1 as (tf & TFPTR & TF).
-        rewrite TFPTR in HFindF. inv HFindF.
-        unfold is_after_call in FACALL1.
-        destruct f0;try contradiction.
-        monadInv TF.
-        unfold is_after_call.
-        
-        unfold trans_function in EQ.
-        destruct (func_no_jmp_rel_dec f0); inversion EQ.
-        monadInv H7.
-        generalize(offsets_after_call_transf_refl (fn_code f0) x0 EQ0).
-        intros EQOfs.
-        simpl. rewrite EQOfs. auto.
-        
-        generalize (Genv.find_funct_ptr_transf_none_partial TRANSF _ FPTR1).
-        intros TPNone.
-        rewrite TPNone in HFindF.
-        inversion HFindF.
         
   + destruct S2. constructor.
 Admitted.
 
 
 
-(* Lemma transf_initial_states: *)
-(*   forall st1, Asm.initial_state prog st1 -> *)
-(*          exists st2, Asm.initial_state tprog st2 /\ match_states Vnullptr st1 st2. *)
-(* Admitted. *)
+Lemma transf_initial_states:
+  forall st1 rs, initial_state prog rs st1 ->
+         exists st2, initial_state tprog rs st2 /\ match_states st1 st2.
+Proof.
+  intros st1 rs HInit.
+  exists st1.
+  inv HInit.
+  split.
+  + econstructor.
+    generalize (Genv.init_mem_transf_partial TRANSF H).
+    eauto.
+    inv H0.
+    econstructor; eauto.
+    rewrite (match_program_main TRANSF); eauto.
+    generalize (Genv.find_symbol_transf_partial TRANSF (prog_main prog)).
+    intros HFind.
+    rewrite <- H1.
+    auto.
+  + destruct st1. constructor.
+Qed.
+
+
+Lemma transf_final_states:
+  forall st1 st2 r,
+  match_states st1 st2 -> final_state st1 r -> final_state st2 r.
+Proof.
+  intros st1 st2 r MS HFinal.
+  inversion HFinal.
+  inversion MS. 
+  econstructor.
+  rewrite <- H1 in H3.
+  inversion H3. auto.
+  rewrite <- H1 in H3.
+  inversion H3.
+  auto.
+Qed.
+
+
+(* Lemma senv_equiv: *)
+(*   Senv.equiv (Genv.genv_senv ge) (Genv.genv_senv tge). *)
+(* Proof. *)
+(*   unfold ge, tge, globalenv. rewrite ! add_globals_genv_senv. simpl. *)
+(*   unfold match_prog in TRANSF. monadInv TRANSF. simpl. *)
+(*   repeat apply conj; auto. *)
+(* Qed. *)
+
+Lemma transf_program_correct:
+  forall rs, forward_simulation (semantics prog rs) (semantics tprog rs).
+Proof.
+  intro rs.
+  eapply forward_simulation_step with match_states.
+  + intros id. unfold match_prog in TRANSF.
+    generalize (Genv.senv_match TRANSF). intros SENV_EQ.
+    red in SENV_EQ.
+    destruct SENV_EQ as (S1 & S2 & S3 & S4). auto.
+  + simpl. intros s1 Hinit.
+    exploit transf_initial_states; eauto.
+  + simpl. intros s1 s2 r MS HFinal. eapply transf_final_states; eauto.
+  + simpl. intros s1 t s1' STEP s2 MS.
+    edestruct step_simulation as (STEP' & MS' ); eauto.
+Qed.
+
+Lemma trans_fun_pres_stacksize: forall f tf,
+    Asmlabelgen.trans_function f = OK tf -> 
+    Asm.fn_stacksize f = Asm.fn_stacksize tf.
+Proof.
+  intros f tf HFunc.
+  unfold trans_function in HFunc.
+  destruct func_no_jmp_rel_dec in HFunc; inversion HFunc.
+  monadInv H0.
+  simpl. auto.
+Qed.
+
 
 End  PRESERVATION.
